WIP: Modified heap and value relation generation and added word array proofs
The first change allows users to pass values and types to the heap
relation and value relation generation to either add or ignore those
types and values for the generation.

Proofs for preservation (update and value semantics), correspondence
and upward propagation between the update and value, and
monomorphisation for them length, get and put methods for word arrays
have been added.

Additional proofs about typing, value typing, monomorphisation and
correspondence in general were also added.

cogent/src/Cogent/Isabelle/CorresSetup.hs
@@ -79,7 +79,7 @@ cHeapTypeClass =
 
 localSetup :: String -> [String]
 localSetup cfile =
-  [ "local_setup \\<open> local_setup_val_rel_type_rel_put_them_in_buckets \"" ++ cfile ++ "\" \\<close>"
+  [ "local_setup \\<open> local_setup_val_rel_type_rel_put_them_in_buckets \"" ++ cfile ++ "\" [] \\<close>"
   , "local_setup \\<open> local_setup_instantiate_cogent_C_heaps_store_them_in_buckets \"" ++ cfile ++ "\" \\<close>"
   ]
 
@@ -105,7 +105,7 @@ locale thy cfile =
   , "  \"heap_rel_ptr = heap_rel_meta is_valid heap\""
   , "  by (simp add: heap_rel_ptr_def[abs_def] heap_rel_meta_def[abs_def])"
   , ""
-  , "local_setup \\<open> local_setup_heap_rel \"" ++ cfile ++ "\" \\<close>"
+  , "local_setup \\<open> local_setup_heap_rel \"" ++ cfile ++ "\" [] [] \\<close>"
   , ""
   , "definition state_rel :: \"((funtyp, abstyp, ptrtyp) store \\<times> lifted_globals) set\""
   , "where"
