cogent/examples/repeat/CorrespondenceHelper.thy
@@ -5,7 +5,7 @@ theory CorrespondenceHelper
     Cogent.Correspondence
 begin 
 
-section "Value relation elimination rules"
+section "Value relation rules"
 
 context correspondence begin
 
@@ -14,7 +14,113 @@ inductive_cases u_v_uprimE     [elim] : "\<Xi>', \<sigma> \<turnstile> UPrim l \
 inductive_cases u_v_r_uemptyE  [elim] : "\<Xi>', \<sigma> \<turnstile>* [] \<sim> vs :r \<tau>s \<langle>r, w\<rangle>"
 inductive_cases u_v_ufunctionE [elim] : "\<Xi>', \<sigma> \<turnstile> UFunction f ts \<sim> v : TFun \<tau> \<rho> \<langle>r, w\<rangle>"
 inductive_cases u_v_uafunE     [elim] : "\<Xi>', \<sigma> \<turnstile> UAFunction f ts \<sim> v : TFun \<tau> \<rho> \<langle>r, w\<rangle>"
-inductive_cases u_v_tfunE      [elim] : "\<Xi>', \<sigma> \<turnstile> u \<sim> v : TFun \<tau> \<rho> \<langle>r, w\<rangle>"
+inductive_cases u_v_uptrE      [elim] : "\<Xi>', \<sigma> \<turnstile> UPtr p rp \<sim> v : \<tau> \<langle>r, w\<rangle>"
+
+inductive_cases u_v_tfunE      : "\<Xi>', \<sigma> \<turnstile> u \<sim> v : TFun \<tau> \<rho> \<langle>r, w\<rangle>"
+inductive_cases u_v_tprimE     : "\<Xi>', \<sigma> \<turnstile> u \<sim> v : TPrim t \<langle>r, w\<rangle>"
+inductive_cases u_v_tconE      : "\<Xi>', \<sigma> \<turnstile> u \<sim> v : TCon a b c \<langle>r, w\<rangle>"
+inductive_cases u_v_tunitE     : "\<Xi>', \<sigma> \<turnstile> u \<sim> v : TUnit \<langle>r, w\<rangle>"
+inductive_cases u_v_tsumE      : "\<Xi>', \<sigma> \<turnstile> u \<sim> v : TSum a \<langle>r, w\<rangle>"
+inductive_cases u_v_tproductE  : "\<Xi>', \<sigma> \<turnstile> u \<sim> v : TProduct a b \<langle>r, w\<rangle>"
+inductive_cases u_v_trecordE   : "\<Xi>', \<sigma> \<turnstile> u \<sim> v : TRecord t s \<langle>r, w\<rangle>"
+inductive_cases u_v_r_temptyE  : "\<Xi>', \<sigma> \<turnstile>* us \<sim> vs :r [] \<langle>r, w\<rangle>"
+
+
+lemma upd_val_rel_record_lengths:
+  "\<Xi>', \<sigma> \<turnstile>* fs \<sim> fs' :r \<tau>s \<langle>r, w\<rangle> \<Longrightarrow> length fs = length fs' \<and> length fs = length \<tau>s"
+  apply (induct fs  arbitrary: fs' \<tau>s r w)
+   apply clarsimp
+   apply (erule u_v_r_uemptyE; simp)
+  apply (erule u_v_r_consE'; clarsimp)
+   apply (elim meta_allE meta_impE, assumption)
+   apply clarsimp
+  apply (elim meta_allE meta_impE, assumption)
+  apply clarsimp
+  done
+
+
+lemma upd_val_rel_record_alt1:
+  "\<Xi>', \<sigma> \<turnstile>* fs \<sim> fs' :r ts \<langle>r, w\<rangle> \<Longrightarrow> 
+      r \<inter> w = {} \<and> length fs = length ts \<and> length fs = length fs' \<and>
+      (\<exists>rs ws. r = \<Union>(set rs) \<and> w = \<Union>(set ws) \<and> length rs = length fs \<and> length ws = length fs \<and>
+        distinct_sets ws \<and>
+        (\<forall>i<length fs. 
+          \<exists>x rp x' n t s. fs ! i = (x, rp) \<and> fs' ! i = x' \<and> ts ! i = (n, t, s) \<and> type_repr t = rp \<and>
+            (s = Taken \<longrightarrow> [] \<turnstile> t wellformed \<and> upd.uval_repr x = rp \<and> upd.uval_repr_deep x = rp \<and> rs ! i = {} \<and> ws ! i = {}) \<and>
+            (s = Present \<longrightarrow> \<Xi>', \<sigma> \<turnstile> x \<sim> x' : t \<langle>rs ! i, ws ! i\<rangle>)))"
+  apply (induct fs arbitrary: fs' ts r w)
+   apply clarsimp
+   apply (erule u_v_r_uemptyE; clarsimp)
+  apply clarsimp
+  apply (case_tac ts; clarsimp)
+   apply (erule u_v_r_temptyE; clarsimp)
+  apply (rename_tac a b fs fs' r w n t s ts)
+  apply (clarsimp simp: upd_val_rel_pointers_noalias)
+  apply (frule upd_val_rel_record_lengths)
+  apply simp
+  apply (case_tac fs'; clarsimp)
+  apply (rename_tac a' fs')
+  apply (drule_tac x = fs' and  y = ts in meta_spec2)
+  apply (case_tac s; clarsimp)
+   apply (drule_tac x = r and y = w in meta_spec2)
+   apply (erule u_v_r_consE; clarsimp)
+   apply (rename_tac fs a' fs' ts t x n rs ws)
+   apply (rule_tac x = "{} # rs" in exI; clarsimp)
+   apply (rule_tac x = "{} # ws" in exI; clarsimp)
+   apply (rename_tac i)
+   apply (case_tac i; clarsimp)
+  apply (erule u_v_r_consE; clarsimp)
+  apply (rename_tac fs a' fs' x t r w ts r' w' n)
+  apply (drule_tac x = r' and y = w' in meta_spec2; clarsimp)
+  apply (rename_tac rs ws)
+  apply (rule_tac x = "r # rs" in exI; clarsimp)
+  apply (rule_tac x = "w # ws" in exI; clarsimp)
+  apply (rename_tac i)
+  apply (case_tac i; clarsimp)
+  done
+
+lemma upd_val_rel_record_alt2:
+  "r \<inter> w = {} \<and> length fs = length ts \<and> length fs = length fs' \<and>
+   (\<exists>rs ws. r = \<Union>(set rs) \<and> w = \<Union>(set ws) \<and> length rs = length fs \<and> length ws = length fs \<and>
+   distinct_sets ws \<and>
+   (\<forall>i<length fs. 
+      \<exists>x rp x' n t s. fs ! i = (x, rp) \<and> fs' ! i = x' \<and> ts ! i = (n, t, s) \<and> type_repr t = rp \<and>
+          (s = Taken \<longrightarrow> [] \<turnstile> t wellformed \<and> upd.uval_repr x = rp \<and> upd.uval_repr_deep x = rp \<and> rs ! i = {} \<and> ws ! i = {}) \<and>
+          (s = Present \<longrightarrow> \<Xi>', \<sigma> \<turnstile> x \<sim> x' : t \<langle>rs ! i, ws ! i\<rangle>)))
+    \<Longrightarrow> \<Xi>', \<sigma> \<turnstile>* fs \<sim> fs' :r ts \<langle>r, w\<rangle>"
+  apply (induct fs arbitrary: fs' ts r w; clarsimp)
+   apply (rule u_v_r_empty)
+  apply (rename_tac a b fs fs' ts rs ws)
+  apply (case_tac ts; clarsimp)
+  apply (rename_tac n t s ts)
+  apply (case_tac fs'; clarsimp)
+  apply (rename_tac a' fs')
+  apply (drule_tac x = fs' and y = ts in meta_spec2; clarsimp)
+  apply (drule_tac x = " \<Union> (set (tl rs))" and y = " \<Union> (set (tl ws))" in meta_spec2)
+  apply (erule meta_impE)
+   apply (rule conjI)
+    apply (erule_tac x = 0 in allE; clarsimp)
+    apply (case_tac rs; clarsimp; case_tac ws; clarsimp)
+    apply blast 
+   apply (rule exI, rule conjI, simp)
+   apply (rule exI, rule conjI, simp)
+   apply (rule conjI; clarsimp)
+   apply (rule conjI)
+    apply (erule_tac x = 0 in allE; clarsimp)
+    apply (case_tac ws; clarsimp)
+    apply clarsimp
+    apply (rename_tac i)
+    apply (erule_tac x = "Suc i" in allE; clarsimp)
+    apply (rule conjI; clarsimp simp: nth_tl)
+   apply (frule_tac x = 0 in allE; simp?; clarsimp)
+  apply (case_tac s; clarsimp)
+   apply (rule u_v_r_cons2; simp?)
+   apply (case_tac rs; clarsimp; case_tac ws; clarsimp)
+  apply (case_tac rs; clarsimp; case_tac ws; clarsimp)
+  apply (rule u_v_r_cons1; simp?)
+   apply blast
+  apply blast
+  done
 
 section "Heap footprint properties"
 
@@ -45,6 +151,15 @@ and   "\<lbrakk> \<Xi>', \<sigma> \<turnstile>* fs \<sim> fs' :r map (\<lambda>(
   apply (clarsimp split: record_state.splits)
   apply (rename_tac a aa ab ac)
   apply (cut_tac K = "[]" and t = ac in bang_kinding_fn; clarsimp)
+  done
+
+lemma u_v_no_heap_no_pointers:
+  "\<lbrakk>no_tvars t; no_theap t; \<Xi>', \<sigma> \<turnstile> u \<sim> v : t \<langle>r, w\<rangle>\<rbrakk> \<Longrightarrow> r = {} \<and> w = {}"
+  apply (frule upd_val_rel_to_uval_typing(1)[THEN upd.uval_typing_to_wellformed(1)])
+  apply (cut_tac K = "[]" and t= t in  no_heap_all_kind; simp?)
+  apply (frule_tac k = UNIV in u_v_escapable_no_readers(1); simp?)
+  apply (frule  u_v_discardable_or_shareable_not_writable(1)[rotated 1]; simp?)
+  apply blast
   done
 
 section "Ordering on abstract function specification properties for abstract function correspondence"
