cogent/examples/repeat/WordArrayAssm.thy
@@ -1,0 +1,10 @@
+theory WordArrayAssm
+  imports
+    WordArray_Abstractions
+    "build/Generated_AllRefine"
+begin
+
+sublocale WordArray \<subseteq> Generated_cogent_shallow _ upd.wa_abs_repr val.wa_abs_typing_v upd.wa_abs_typing_u wa_abs_upd_val
+  by (unfold_locales)
+
+end
